Start work on reduction step

ironfleet/src/Dafny/Distributed/Concur/Reduction.i.dfy
@@ -1,8 +1,10 @@
+include "../Common/Collections/Seqs.i.dfy"
 include "Refinement.i.dfy"
 
 module ReductionModule
 {
     import opened RefinementModule
+    import opened Collections__Seqs_i
 
     predicate SpecBehaviorStuttersForMoversInTrace(trace:Trace, sb:seq<SpecState>)
     {
@@ -39,10 +41,16 @@ module ReductionModule
                         && t[endPos].EntryEndGroup?
                         && (forall i :: 0 < i < endPos ==> t[i].EntryAction?)
                         && (forall i :: 0 <= i <= endPos ==> GetEntryLevel(t[i]) == level)
+                        && t[endPos].coarse_level > level
                         && EntriesCompatibleWithReduction(t[1..endPos])
                         && EntriesReducibleToEntry(t[1..endPos], t[endPos].reduced_entry)
                         && ActorTraceCompatibleWithReduction(t[endPos+1..], level)
            )
+    }
+
+    predicate ActorTraceDoneWithReduction(t:Trace, level:int)
+    {
+        forall e :: e in t ==> GetEntryLevel(e) > level
     }
 
     lemma lemma_IfEntriesCompatibleWithReductionAndOneIsntRightMoverThenRestAreLeftMovers(entries:seq<Entry>, i:int, j:int)
@@ -77,33 +85,32 @@ module ReductionModule
         }
     }
 
-
-    lemma PerformOneReductionSwap(
+/*
+    lemma lemma_PerformOneReductionSwap(
         trace:Trace,
         db:seq<DistributedSystemState>,
-        firstEntryPos:int
+        first_entry_pos:int
         ) returns (
         trace':Trace,
         db':seq<DistributedSystemState>
         )
         requires IsValidDistributedSystemTraceAndBehavior(trace, db);
-        requires 0 <= firstEntryPos < |trace| - 1;
-        requires GetEntryActor(trace[firstEntryPos]) != GetEntryActor(trace[firstEntryPos+1]);
-        requires EntryIsRightMover(trace[firstEntryPos]) || EntryIsLeftMover(trace[firstEntryPos+1]);
+        requires 0 <= first_entry_pos < |trace| - 1;
+        requires GetEntryActor(trace[first_entry_pos]) != GetEntryActor(trace[first_entry_pos+1]);
+        requires EntryIsRightMover(trace[first_entry_pos]) || EntryIsLeftMover(trace[first_entry_pos+1]);
         ensures  IsValidDistributedSystemTraceAndBehavior(trace', db');
-        ensures  trace' == trace[firstEntryPos := trace[firstEntryPos+1]][firstEntryPos + 1 := trace[firstEntryPos]];
         ensures  forall sb' :: DistributedSystemBehaviorRefinesSpecBehavior(db', sb') && SpecBehaviorStuttersForMoversInTrace(trace', sb')
                      ==> exists sb :: DistributedSystemBehaviorRefinesSpecBehavior(db, sb) && SpecBehaviorStuttersForMoversInTrace(trace, sb);
     {
-        var entry1 := trace[firstEntryPos];
-        var entry2 := trace[firstEntryPos+1];
-        var ds1 := db[firstEntryPos];
-        var ds2 := db[firstEntryPos+1];
-        var ds3 := db[firstEntryPos+2];
+        var entry1 := trace[first_entry_pos];
+        var entry2 := trace[first_entry_pos+1];
+        var ds1 := db[first_entry_pos];
+        var ds2 := db[first_entry_pos+1];
+        var ds3 := db[first_entry_pos+2];
 
-        trace' := trace[firstEntryPos := entry2][firstEntryPos + 1 := entry1];
+        trace' := trace[first_entry_pos := entry2][first_entry_pos + 1 := entry1];
         var ds2' := lemma_MoverCommutativityForEntries(entry1, entry2, ds1, ds2, ds3);
-        db' := db[firstEntryPos + 1 := ds2'];
+        db' := db[first_entry_pos + 1 := ds2'];
 
         forall sb' | DistributedSystemBehaviorRefinesSpecBehavior(db', sb') && SpecBehaviorStuttersForMoversInTrace(trace', sb')
             ensures exists sb :: DistributedSystemBehaviorRefinesSpecBehavior(db, sb) && SpecBehaviorStuttersForMoversInTrace(trace, sb);
@@ -111,22 +118,225 @@ module ReductionModule
             var sb:seq<SpecState>;
             if EntryIsRightMover(entry1)
             {
-                assert sb'[firstEntryPos+1] == sb'[firstEntryPos+2];
-                sb := sb'[firstEntryPos + 1 := sb'[firstEntryPos]];
+                assert sb'[first_entry_pos+1] == sb'[first_entry_pos+2];
+                sb := sb'[first_entry_pos + 1 := sb'[first_entry_pos]];
                 assert SpecBehaviorStuttersForMoversInTrace(trace, sb);
-                lemma_RightMoverForwardPreservation(entry1, ds1, ds2, sb[firstEntryPos]);
+                lemma_RightMoverForwardPreservation(entry1, ds1, ds2, sb[first_entry_pos]);
                 assert DistributedSystemBehaviorRefinesSpecBehavior(db, sb);
             }
             else
             {
                 assert EntryIsLeftMover(entry2);
-                assert sb'[firstEntryPos] == sb'[firstEntryPos+1];
-                sb := sb'[firstEntryPos + 1 := sb'[firstEntryPos+2]];
+                assert sb'[first_entry_pos] == sb'[first_entry_pos+1];
+                sb := sb'[first_entry_pos + 1 := sb'[first_entry_pos+2]];
                 assert SpecBehaviorStuttersForMoversInTrace(trace, sb);
-                lemma_LeftMoverBackwardPreservation(entry2, ds2, ds3, sb[firstEntryPos+1]);
+                lemma_LeftMoverBackwardPreservation(entry2, ds2, ds3, sb[first_entry_pos+1]);
                 assert DistributedSystemBehaviorRefinesSpecBehavior(db, sb);
             }
             assert DistributedSystemBehaviorRefinesSpecBehavior(db, sb) && SpecBehaviorStuttersForMoversInTrace(trace, sb);
+        }
+    }
+*/
+
+    lemma lemma_PerformMoveRight(
+        trace:Trace,
+        db:seq<DistributedSystemState>,
+        first_entry_pos:int
+        ) returns (
+        trace':Trace,
+        db':seq<DistributedSystemState>
+        )
+        requires IsValidDistributedSystemTraceAndBehavior(trace, db);
+        requires 0 <= first_entry_pos < |trace| - 1;
+        requires GetEntryActor(trace[first_entry_pos]) != GetEntryActor(trace[first_entry_pos+1]);
+        requires EntryIsRightMover(trace[first_entry_pos]);
+        ensures  IsValidDistributedSystemTraceAndBehavior(trace', db');
+        ensures  |db'| == |db|;
+        ensures  forall sb' :: DistributedSystemBehaviorRefinesSpecBehavior(db', sb') && sb'[first_entry_pos+1] == sb'[first_entry_pos+2]
+                     ==> exists sb :: DistributedSystemBehaviorRefinesSpecBehavior(db, sb) && sb[first_entry_pos] == sb[first_entry_pos+1];
+    {
+        var entry1 := trace[first_entry_pos];
+        var entry2 := trace[first_entry_pos+1];
+        var ds1 := db[first_entry_pos];
+        var ds2 := db[first_entry_pos+1];
+        var ds3 := db[first_entry_pos+2];
+
+        trace' := trace[first_entry_pos := entry2][first_entry_pos + 1 := entry1];
+        var ds2' := lemma_MoverCommutativityForEntries(entry1, entry2, ds1, ds2, ds3);
+        db' := db[first_entry_pos + 1 := ds2'];
+
+        forall sb' | DistributedSystemBehaviorRefinesSpecBehavior(db', sb') && sb'[first_entry_pos+1] == sb'[first_entry_pos+2]
+            ensures exists sb :: DistributedSystemBehaviorRefinesSpecBehavior(db, sb) && sb[first_entry_pos] == sb[first_entry_pos+1];
+        {
+            var sb := sb'[first_entry_pos + 1 := sb'[first_entry_pos]];
+            lemma_RightMoverForwardPreservation(entry1, ds1, ds2, sb[first_entry_pos]);
+            assert DistributedSystemBehaviorRefinesSpecBehavior(db, sb);
+            assert sb[first_entry_pos] == sb[first_entry_pos+1];
+        }
+    }
+
+    lemma lemma_PerformMoveLeft(
+        trace:Trace,
+        db:seq<DistributedSystemState>,
+        first_entry_pos:int
+        ) returns (
+        trace':Trace,
+        db':seq<DistributedSystemState>
+        )
+        requires IsValidDistributedSystemTraceAndBehavior(trace, db);
+        requires 0 <= first_entry_pos < |trace| - 1;
+        requires GetEntryActor(trace[first_entry_pos]) != GetEntryActor(trace[first_entry_pos+1]);
+        requires EntryIsLeftMover(trace[first_entry_pos+1]);
+        ensures  IsValidDistributedSystemTraceAndBehavior(trace', db');
+        ensures  |db'| == |db|;
+        ensures  forall sb' :: DistributedSystemBehaviorRefinesSpecBehavior(db', sb') && sb'[first_entry_pos] == sb'[first_entry_pos+1]
+                     ==> exists sb :: DistributedSystemBehaviorRefinesSpecBehavior(db, sb) && sb[first_entry_pos+1] == sb[first_entry_pos+2];
+    {
+        var entry1 := trace[first_entry_pos];
+        var entry2 := trace[first_entry_pos+1];
+        var ds1 := db[first_entry_pos];
+        var ds2 := db[first_entry_pos+1];
+        var ds3 := db[first_entry_pos+2];
+
+        trace' := trace[first_entry_pos := entry2][first_entry_pos + 1 := entry1];
+        var ds2' := lemma_MoverCommutativityForEntries(entry1, entry2, ds1, ds2, ds3);
+        db' := db[first_entry_pos + 1 := ds2'];
+
+        forall sb' | DistributedSystemBehaviorRefinesSpecBehavior(db', sb') && sb'[first_entry_pos] == sb'[first_entry_pos+1]
+            ensures exists sb :: DistributedSystemBehaviorRefinesSpecBehavior(db, sb) && sb[first_entry_pos+1] == sb[first_entry_pos+2];
+        {
+            var sb := sb'[first_entry_pos + 1 := sb'[first_entry_pos+2]];
+            lemma_LeftMoverBackwardPreservation(entry2, ds2, ds3, sb[first_entry_pos+1]);
+            assert DistributedSystemBehaviorRefinesSpecBehavior(db, sb);
+            assert sb[first_entry_pos+1] == sb[first_entry_pos+2];
+        }
+    }
+
+    lemma lemma_AddStuttersForReductionStep(
+        trace:Trace,
+        db:seq<DistributedSystemState>,
+        begin_entry_pos:int,
+        end_entry_pos:int,
+        pivot:int,
+        trace':Trace,
+        db':seq<DistributedSystemState>,
+        sb':seq<SpecState>
+        ) returns (
+        sb:seq<SpecState>
+        )
+        requires IsValidDistributedSystemTraceAndBehavior(trace, db);
+        requires 0 <= begin_entry_pos < end_entry_pos < |trace|;
+        requires trace[begin_entry_pos].EntryBeginGroup?;
+        requires trace[end_entry_pos].EntryEndGroup?;
+        requires EntriesCompatibleWithReductionUsingPivot(trace[begin_entry_pos+1 .. end_entry_pos], pivot);
+        requires IsValidDistributedSystemTraceAndBehavior(trace', db');
+        requires DistributedSystemBehaviorRefinesSpecBehavior(db', sb');
+        requires trace' == trace[..begin_entry_pos] + [trace[end_entry_pos].reduced_entry] + trace[end_entry_pos+1 ..];
+        requires db' == db[..begin_entry_pos+1] + db[end_entry_pos+1 ..];
+
+        ensures  DistributedSystemBehaviorRefinesSpecBehavior(db, sb);
+        ensures  forall i :: begin_entry_pos <= i <= end_entry_pos && i != begin_entry_pos + 1 + pivot ==> sb[i] == sb[i+1];
+    {
+        var entries := trace[begin_entry_pos+1 .. end_entry_pos];
+        var ss := sb'[begin_entry_pos];
+        var ss' := sb'[begin_entry_pos+1];
+
+        var pivot_pos := begin_entry_pos + 1 + pivot;
+        assert pivot_pos <= end_entry_pos;
+
+        sb := sb'[..begin_entry_pos+1];
+
+        while |sb| <= pivot_pos
+            invariant begin_entry_pos + 1 <= |sb| <= pivot_pos + 1;
+            invariant forall i :: 0 <= i < begin_entry_pos + 1 ==> sb[i] == sb'[i];
+            invariant forall i :: begin_entry_pos + 1 <= i < |sb| ==> sb[i] == ss;
+            invariant last(sb) == ss;
+            invariant forall i :: begin_entry_pos <= i < |sb| - 1 ==> sb[i] == sb[i+1];
+            invariant IsValidSpecBehavior(sb);
+        {
+            sb := sb + [ss];
+        }
+
+        sb := sb + [ss'];
+        assert |sb| == pivot_pos + 2;
+
+        while |sb| < end_entry_pos + 2
+            invariant pivot_pos + 2 <= |sb| <= end_entry_pos + 2;
+            invariant forall i :: 0 <= i < begin_entry_pos + 1 ==> sb[i] == sb'[i];
+            invariant forall i :: begin_entry_pos + 1 <= i <= pivot_pos ==> sb[i] == ss;
+            invariant forall i :: pivot_pos < i < |sb| ==> sb[i] == ss';
+            invariant last(sb) == ss';
+            invariant forall i :: begin_entry_pos <= i < |sb| - 1 && i != begin_entry_pos + 1 + pivot ==> sb[i] == sb[i+1];
+            invariant IsValidSpecBehavior(sb);
+        {
+            sb := sb + [ss'];
+        }
+
+        assert forall i :: begin_entry_pos <= i <= end_entry_pos && i != begin_entry_pos + 1 + pivot ==> sb[i] == sb[i+1];
+
+        ghost var prev_sb := sb;
+        sb := sb + sb'[begin_entry_pos+2..];
+        forall i | 0 <= i < |sb| - 1
+            ensures SpecNext(sb[i], sb[i+1]) || sb[i] == sb[i+1];
+        {
+            if i < |prev_sb| - 1 {
+            }
+            else if i == |prev_sb| - 1 {
+                assert SpecNext(last(prev_sb), sb'[begin_entry_pos+2]) || last(prev_sb) == sb'[begin_entry_pos+2];
+            }
+            else {
+            }
+        }
+
+        assert IsValidSpecBehavior(sb);
+        assume DistributedSystemBehaviorRefinesSpecBehavior(db, sb);
+    }
+
+    lemma lemma_PerformOneReductionStep(
+        trace:Trace,
+        db:seq<DistributedSystemState>,
+        actor:Actor,
+        level:int,
+        begin_entry_pos:int,
+        end_entry_pos:int,
+        pivot:int
+        ) returns (
+        trace':Trace,
+        db':seq<DistributedSystemState>
+        )
+        requires IsValidDistributedSystemTraceAndBehavior(trace, db);
+        requires 0 <= begin_entry_pos < end_entry_pos < |trace|;
+        requires trace[begin_entry_pos].EntryBeginGroup?;
+        requires trace[end_entry_pos].EntryEndGroup?;
+        requires forall i :: begin_entry_pos < i < end_entry_pos ==> trace[i].EntryAction?;
+        requires forall i :: begin_entry_pos <= i <= end_entry_pos ==> GetEntryActor(trace[i]) == actor;
+        requires forall i :: begin_entry_pos <= i <= end_entry_pos ==> GetEntryLevel(trace[i]) == level;
+        requires EntriesCompatibleWithReductionUsingPivot(trace[begin_entry_pos+1 .. end_entry_pos], pivot);
+        requires EntriesReducibleToEntry(trace[begin_entry_pos+1 .. end_entry_pos], trace[end_entry_pos].reduced_entry);
+        ensures  IsValidDistributedSystemTraceAndBehavior(trace', db');
+        ensures  forall sb' :: DistributedSystemBehaviorRefinesSpecBehavior(db', sb')
+                     ==> exists sb :: DistributedSystemBehaviorRefinesSpecBehavior(db, sb);
+    {
+        var entries := trace[begin_entry_pos+1 .. end_entry_pos];
+        var reduced_entry := trace[end_entry_pos].reduced_entry;
+        trace' := trace[..begin_entry_pos] + [reduced_entry] + trace[end_entry_pos+1 ..];
+        db' := db[..begin_entry_pos+1] + db[end_entry_pos+1 ..];
+
+        var tiny_db := db[begin_entry_pos+1 .. end_entry_pos+1];
+        assert |tiny_db| == |entries| + 1;
+        assert forall i :: 0 <= i < |entries| ==> DistributedSystemNextEntryAction(tiny_db[i], tiny_db[i+1], entries[i]);
+        assert DistributedSystemNextEntryAction(tiny_db[0], tiny_db[|entries|], reduced_entry);
+
+        assert db[begin_entry_pos] == db[begin_entry_pos+1];
+        assert db[end_entry_pos] == db[end_entry_pos+1];
+        assert DistributedSystemNextEntryAction(db'[begin_entry_pos], db'[begin_entry_pos+1], reduced_entry);
+        assert IsValidDistributedSystemTraceAndBehavior(trace', db');
+
+        forall sb' | DistributedSystemBehaviorRefinesSpecBehavior(db', sb')
+            ensures exists sb :: DistributedSystemBehaviorRefinesSpecBehavior(db, sb) &&
+                            forall i :: begin_entry_pos <= i <= end_entry_pos && i != begin_entry_pos + 1 + pivot ==> sb[i] == sb[i+1];
+        {
+            var sb := lemma_AddStuttersForReductionStep(trace, db, begin_entry_pos, end_entry_pos, pivot, trace', db', sb');
         }
     }
 
